separation.v
@@ -1,5 +1,5 @@
-Require Import Events.
-Require Import TraceModel.
+Require Import Events. 
+Require Import TraceModel. 
 Require Import Properties.
 Require Import CommonST.
 Require Import Robustdef.
@@ -17,151 +17,191 @@ Definition ϕ_ctx  := prod nat (ctx L).
 Definition ϕ_plug : ϕ_par -> ϕ_ctx -> ϕ_prg :=
   fun P C =>  (fst C , plug L P (snd C)).
 
-Definition length (m : finpref) : nat :=
-  match m with
-  | fstop m _ => List.length m
-  | ftbd m  => List.length m
-  end.
+Lemma omega_fact : forall n m, n <= m -> (S n) <= (S m).
+Proof. intros n m h. omega. Qed.
 
-Lemma stop_same_lenght: forall m es, length m = length (m[fstop es/ftbd]).
+Fixpoint take_n_of_stream {A: Type} (s : stream) (n : nat) : list A :=
+  match n, s with
+  | 0, _  => nil
+  | S m, scons a s' => cons a (take_n_of_stream s' m)
+  end. 
+
+Lemma take_n_of_stream_prefix {A : Type} (s : stream) (n: nat) :
+  @list_stream_prefix A (take_n_of_stream s n) s.  
 Proof.
-  now destruct m.
+  generalize dependent s. induction n; try now auto. 
+  intros []; simpl. now auto.  
 Qed.
 
-Fixpoint take_n (t : trace) (n : nat) : trace :=
-  match n, t with
-  | _ ,tstop es     => tstop es
-  | 0, _            => tstop an_endstate
-  | _, tsilent      => tsilent
-  | S m, tcons x xs => tcons x (take_n xs m)
-  end.                               
-
-Fixpoint take_nth_pref' (t : trace) (n : nat) : pref :=
-  match n, t with
-  | 0, _  | _, tstop _ | _, tsilent => nil
-  | S m, tcons x xs => cons x (take_nth_pref' xs m)
+Lemma take_n_of_stream_length {A : Type} (s: stream) (n: nat) :
+  @length A (take_n_of_stream s n) <= n. 
+Proof.
+  generalize dependent s. induction n; try now auto.
+  intros []; simpl; auto. apply omega_fact. now apply IHn.
+Qed. 
+  
+Fixpoint take_n_of_list {A : Type} (l : list A) (n : nat) : list A :=
+  match n, l with
+  | 0, _ | _, nil => nil
+  | S m, cons x xs => cons x (take_n_of_list xs m)
   end.
 
-Definition take_nth_pref (t : trace) (n : nat) : finpref :=
-  ftbd (take_nth_pref' t n).
+Lemma take_n_of_list_prefix {A : Type} (l : list A) (n : nat) :
+  list_list_prefix (take_n_of_list l n) l.
+Proof.
+  generalize dependent l. induction n; try now auto;
+  intros []; simpl; try now auto. 
+Qed.
+
+Lemma take_n_of_list_length {A : Type} (l : list A) (n : nat) :
+  length (take_n_of_list l n) <= n.
+Proof.
+  generalize dependent l. induction n; try now auto.
+  intros []; simpl; auto.
+  intros []; simpl; auto. 
+  omega. apply omega_fact. now apply IHn.
+Qed.   
+             
+Definition take_n (t : trace) (n : nat) : list event :=
+  match t with
+  | tstop l _ | tsilent l => take_n_of_list l n 
+  | tstream s             => take_n_of_stream s n
+  end.
+
+Lemma take_n_prefix (t : trace) (n: nat) :
+  prefix (ftbd (take_n t n)) t.
+Proof.
+  destruct t; 
+    [ now apply take_n_of_list_prefix
+    | now apply take_n_of_list_prefix
+    | now apply take_n_of_stream_prefix].       
+Qed.
+
+Lemma take_n_lenght (t : trace) (n : nat): length (take_n t n) <= n.
+Proof.
+  destruct t;
+    [ now apply take_n_of_list_length
+    | now apply take_n_of_list_length
+    | now apply take_n_of_stream_length].
+Qed.
+  
+Lemma list_list_prefix_shorter {A : Type} : forall l1 l2 : list A,
+  list_list_prefix l1 l2 -> length l1 <= length l2.
+Proof.
+  induction l1; intros l2 Hpref.
+  + simpl. omega.
+  + destruct l2; inversion Hpref; subst. simpl.
+    apply omega_fact. now apply IHl1.
+Qed. 
+
 
 (* Fixpoint take_nth_pref (t : trace) (n : nat) : finpref := *)
 (*   match n, t with *)
 (*   | 0, _ | _ ,tstop | _, tsilent => ftbd *)
 (*   | S m, tcons x xs => fcons x (take_nth_pref xs m) *)
-(*   end. *)                               
+(*   end.                            *)    
 
-Lemma nth_pref_pref : forall t n, prefix (take_nth_pref t n) t.
-Proof.
-  intros t n. generalize dependent t. induction n; intros t; try now auto.
-  destruct t; simpl in *; try now auto. 
-Qed. 
+(* Lemma nth_pref_pref : forall t n, prefix (take_nth_pref t n) t. *)
+(* Proof. *)
+(*   intros t n. generalize dependent t. induction n; intros t; try now auto. *)
+(*   destruct t; simpl in *; try now auto.  *)
+(* Qed.  *)
 
-Lemma pref_take_pref : forall m t,
-    prefix m t ->
-    prefix m (take_n t (length m)).
-Proof.
-  intros m t. generalize dependent t. destruct m as [m | m]; induction m; intros t hpref; try now auto.
-  + destruct t; try now auto.
-  + destruct t; try now auto.
-    simpl in *. destruct hpref as [h1 h2]. split; try now auto.
-  + destruct t; try now auto.
-    simpl in *; destruct hpref as [h1 h2]. split; try now auto.
-Qed.   
+(* Lemma pref_take_pref : forall m t, *)
+(*     prefix m t -> *)
+(*     prefix m (take_n t (length m)). *)
+(* Proof. *)
+(*   intros m t. generalize dependent t. destruct m as [m | m]; induction m; intros t hpref; try now auto. *)
+(*   + destruct t; try now auto. *)
+(*   + destruct t; try now auto. *)
+(*     simpl in *. destruct hpref as [h1 h2]. split; try now auto. *)
+(*   + destruct t; try now auto. *)
+(*     simpl in *; destruct hpref as [h1 h2]. split; try now auto. *)
+(* Qed.    *)
 
-Lemma take_embedding : forall t m,
-    prefix m t ->
-    exists es, (take_n t (length m)) = embedding es m.
-Proof.
-  intros t m. generalize dependent t.
-  destruct m as [m | m]; induction m; intros t hpref; simpl in *;
-    destruct t; subst; try now eauto.
-  - destruct hpref as [h1 h2]; subst.
-    specialize (IHm t h2). destruct IHm as [es Hes]. now rewrite Hes.
-  - destruct hpref as [h1 h2]; subst.
-    destruct (IHm t h2) as [es Hes]. eexists; now rewrite Hes.
-Qed. 
+(* Lemma take_embedding : forall t m, *)
+(*     prefix m t -> *)
+(*     exists es, (take_n t (length m)) = embedding es m. *)
+(* Proof. *)
+(*   intros t m. generalize dependent t. *)
+(*   destruct m as [m | m]; induction m; intros t hpref; simpl in *; *)
+(*     destruct t; subst; try now eauto. *)
+(*   - destruct hpref as [h1 h2]; subst. *)
+(*     specialize (IHm t h2). destruct IHm as [es Hes]. now rewrite Hes. *)
+(*   - destruct hpref as [h1 h2]; subst. *)
+(*     destruct (IHm t h2) as [es Hes]. eexists; now rewrite Hes. *)
+(* Qed.  *)
 
 Definition ϕ_sem : ϕ_prg -> prop :=
   fun P =>
   (fun t : trace =>
-     exists m es, t = embedding es m /\ psem (snd P) m /\ length m <= (fst P)).
+     exists l es, t = tstop l es  /\ psem (snd P) (ftbd l) /\ length l <= (fst P)).
 
-Lemma omega_fact : forall n m, n <= m -> (S n) <= (S m).
-Proof. intros n m h. omega. Qed.
+  
+(*   intros n. induction n; intros t; try now auto. *)
+(*   destruct t; simpl; try now auto. *)
+(*   + omega. *)
+(*   + omega. *)
+(*   + apply omega_fact. now apply IHn. *)
+(* Qed. *)
 
-Lemma length_take_n : forall n t,
-    length (take_nth_pref t n) <= n.
-Proof.
-  intros n. induction n; intros t; try now auto.
-  destruct t; simpl; try now auto.
-  + omega.
-  + omega.
-  + apply omega_fact. now apply IHn.
-Qed.
-
-Lemma length_smaller : forall P t,
-    sem L (snd P) t -> length (take_nth_pref t (fst P)) <= fst P.
-Proof.
-  intros P t hsem. now apply length_take_n.
-Qed.
+(* Lemma length_smaller : forall P t, *)
+(*     sem L (snd P) t -> length (take_nth_pref t (fst P)) <= fst P. *)
+(* Proof. *)
+(*   intros P t hsem. now apply length_take_n. *)
+(* Qed. *)
 
 Lemma non_empty_ϕ : forall P, exists t, ϕ_sem P t.
 Proof.
-  intros P. destruct (non_empty_sem L (snd P)) as [t h].
-  exists (embedding an_endstate (take_nth_pref t (fst P))). unfold ϕ_sem.
-  exists (take_nth_pref t (fst P)). repeat (split; try now auto).
-  unfold psem. exists an_endstate.
-  split.
-  + reflexivity.
-  + split.
-    ++ exists t. split; try now auto. now apply nth_pref_pref.
-    ++ now apply length_smaller.
+  intros [n Pl].
+  destruct (non_empty_sem L Pl) as [t HsemL]. 
+  exists (tstop (take_n t n) an_endstate). unfold ϕ_sem.
+  exists (take_n t n), an_endstate. simpl. repeat (split; try now auto).
+  exists t. split; try now auto.   
+  + now apply take_n_prefix.
+  + now apply take_n_lenght. 
 Qed.
 
-Lemma fpr_shorter: forall m1 m2, fpr m1 m2 -> length m1 <= length m2.
-Proof.
-  destruct m1 as [m1 | m1]; induction m1; intros m2 hpref; simpl; try omega.
-  + destruct m2; try now auto. inversion hpref; subst.
-    simpl. apply omega_fact. omega.
-  + destruct m2 as [m2 | m2]; destruct m2; try now auto.
-    ++ simpl. inversion hpref; subst.
-       apply omega_fact. now apply (IHm1 (fstop m2 an_endstate) H0).
-    ++ simpl. inversion hpref; subst.
-       apply omega_fact. now apply (IHm1 (ftbd m2) H0).
-Qed.
+(* Lemma fpr_shorter: forall m1 m2, fpr m1 m2 -> length m1 <= length m2. *)
+(* Proof. *)
+(*   destruct m1 as [m1 | m1]; induction m1; intros m2 hpref; simpl; try omega. *)
+(*   + destruct m2; try now auto. inversion hpref; subst. *)
+(*     simpl. apply omega_fact. omega. *)
+(*   + destruct m2 as [m2 | m2]; destruct m2; try now auto. *)
+(*     ++ simpl. inversion hpref; subst. *)
+(*        apply omega_fact. now apply (IHm1 (fstop m2 an_endstate) H0). *)
+(*     ++ simpl. inversion hpref; subst. *)
+(*        apply omega_fact. now apply (IHm1 (ftbd m2) H0). *)
+(* Qed. *)
   
-(*TODO : move to Tracemdel.v *)         
-Lemma prefix_embeding_fpr : forall m1 m2 es,
-    prefix m1 (embedding es m2) -> fpr m1 (m2[fstop es/ftbd]).
-Proof.
-  destruct m1 as [m1 | m1]; induction m1; intros [m2 | m2]; intros es hpref; try now auto;
-    try now destruct m2.
-  + destruct m2; try now auto. inversion hpref. subst.
-    simpl. specialize (IHm1 (fstop m2 e0) e H0). destruct IHm1; now subst.
-  + destruct m2; try now auto. inversion hpref. subst.
-    simpl. specialize (IHm1 (fstop m2 es) e H0). destruct IHm1; now subst.
-  + destruct m2; try now auto. inversion hpref. subst.
-    simpl. specialize (IHm1 (fstop m2 e) es H0). simpl in *; now subst.  
-  + destruct m2; try now auto. inversion hpref. subst.
-    simpl. specialize (IHm1 (fstop m2 es) es H0). simpl in *; now subst.
-Qed.
+(* (*TODO : move to Tracemdel.v *)          *)
+(* Lemma prefix_embeding_fpr : forall m1 m2 es, *)
+(*     prefix m1 (embedding es m2) -> fpr m1 (m2[fstop es/ftbd]). *)
+(* Proof. *)
+(*   destruct m1 as [m1 | m1]; induction m1; intros [m2 | m2]; intros es hpref; try now auto; *)
+(*     try now destruct m2. *)
+(*   + destruct m2; try now auto. inversion hpref. subst. *)
+(*     simpl. specialize (IHm1 (fstop m2 e0) e H0). destruct IHm1; now subst. *)
+(*   + destruct m2; try now auto. inversion hpref. subst. *)
+(*     simpl. specialize (IHm1 (fstop m2 es) e H0). destruct IHm1; now subst. *)
+(*   + destruct m2; try now auto. inversion hpref. subst. *)
+(*     simpl. specialize (IHm1 (fstop m2 e) es H0). simpl in *; now subst.   *)
+(*   + destruct m2; try now auto. inversion hpref. subst. *)
+(*     simpl. specialize (IHm1 (fstop m2 es) es H0). simpl in *; now subst. *)
+(* Qed. *)
 
 Lemma leq_trans : forall n1 n2 n3, n1 <= n2 -> n2 <= n3 -> n1 <= n3.
 Proof. intros n1 n2 n3 h1 h2. omega. Qed.
 
 (* intuition there in t in sem longer than m *)
-Lemma psem_consequence : forall C P t m,
+Lemma psem_consequence : forall C P t l,
     ϕ_sem (ϕ_plug P C) t ->
-    prefix m t ->
-    length m <= fst C.
+    prefix (ftbd l) t ->
+    length l <= fst C.
 Proof.
-  intros C P t m [mm [es [hem [h1 h2]]]] hpref. simpl in *.
-  rewrite stop_same_lenght with (es := es)in h2 .
-  apply (leq_trans (length m) (length(mm[fstop es/ftbd])) (fst C)); try now auto.
-  apply fpr_shorter; try now auto.
-  rewrite embedding_is_the_same in hem. rewrite hem in hpref.
-  apply prefix_embeding_fpr. now rewrite embedding_is_the_same.
+  intros [n C] P t m [mm [es [hem [h1 h2]]]] hpref. subst. 
+  simpl in *. apply (leq_trans (length m) (length mm) n); auto.   
+  now apply list_list_prefix_shorter.   
 Qed.
 
 Definition ϕ := Build_language ϕ_plug
@@ -185,15 +225,20 @@ Proof.
   unfold rsat. repeat rewrite not_forall_ex_not.
   intros [C hC]. unfold sat in *. rewrite not_forall_ex_not in *.
   destruct hC as [t hh]. rewrite not_imp in hh.
-  destruct hh as [h1 h2]. destruct (Hsafety t h2) as [m [hpref hwit]].
-  exists (length m, C). intros ff. simpl in ff.
-  specialize (hwit (take_n t (length m))). apply hwit.
-  now apply pref_take_pref. apply ff. unfold ϕ_sem, ϕ_plug.
-  exists m. repeat (split; simpl; try now auto).
-  pose proof (take_embedding t m hpref).
-  destruct H as [es Hes].
-  exists es. repeat (split; simpl in *; try now auto).
-  now exists t.
+  destruct hh as [h1 h2]. destruct (Hsafety t h2) as [m [hpref hwit]]. 
+  destruct m.
+  + exists (length l, C). intros ff. simpl in ff.
+    destruct t; inversion hpref; subst.
+    apply (hwit (tstop l0 e)); auto.
+    apply ff. unfold ϕ_sem, ϕ_plug; simpl. 
+    exists l0, e. repeat (split; try now auto).
+    exists (tstop l0 e). split; auto. simpl. now apply list_list_prefix_ref. 
+  + exists (length l, C). intros ff. simpl in ff.
+    apply (hwit (tstop l an_endstate)); auto.
+    simpl. now apply list_list_prefix_ref.   
+    apply ff. unfold ϕ_sem, ϕ_plug; simpl.
+    exists l, an_endstate. repeat (split; try now auto).
+    now exists t. 
 Qed.
 
 (*
@@ -201,41 +246,43 @@ Qed.
    an_envet;
   END.
  *)
-Definition an_omega := constant_trace (an_event).
-Definition another_omega := constant_trace (another_event).
+Definition an_omega := constant_stream (an_event).
+Definition another_omega := constant_stream (another_event).
 
-Hypothesis an_omega_produced : exists P, forall C, sem L (plug L P C) an_omega.
-Hypothesis another_omega_produced : exists P, forall C, sem L (plug L P C) another_omega.
+Hypothesis an_omega_produced : exists P, forall C, sem L (plug L P C) (tstream an_omega).
+Hypothesis another_omega_produced : exists P, forall C, sem L (plug L P C) (tstream another_omega).
 
-Lemma not_equal: ~ t_eq an_omega another_omega.
-Proof.
-  rewrite neq_finitely_refutable.
-  exists (ftbd (cons an_event nil)), (ftbd (cons another_event nil)).
+Lemma not_equal: ~ stream_eq an_omega another_omega.
+Proof.   
+  rewrite stream_eq_finetely_refutable. 
+  exists nil, an_event, another_event. 
   repeat (split; try now auto).
-  intros [f1 f2]. inversion f1. now apply different_events.
+  now apply different_events.
 Qed.
 
-Definition my_pi := fun t => fin t \/ t_eq t an_omega.
+Definition my_pi :=
+  fun t =>
+    match t with
+    | tstop _ _ => True
+    | tstream s  => stream_eq s an_omega
+    | _ => False
+    end. 
 
 Lemma my_pi_liveness : Liveness my_pi.
 Proof.
-  apply all_fin_in_all_liv. unfold my_pi.
-  now auto.
+  apply all_fin_in_all_liv. intros t Hfin. destruct t; now inversion Hfin. 
 Qed.
 
-Lemma another_omega_not_in_my_pi : ~ my_pi another_omega.
+Lemma another_omega_not_in_my_pi : ~ my_pi (tstream another_omega).
 Proof.
- intros [K1 | K2].
- + assert (inf another_omega) by now apply inf_constant_trace.
-   now auto.
- + apply t_eq_symm in K2. now apply not_equal.
+ simpl. intros H.  apply stream_eq_sym in H. now apply not_equal. 
 Qed.
 
 Lemma cut_lemma : forall C P t, sem ϕ (plug ϕ P C) t -> fin t.
 Proof.
   intros C P t H. simpl in*.
-  unfold ϕ_sem, ϕ_plug in *. destruct H as [m [es [hp H]]]. rewrite hp.
-  now apply embed_fin.
+  unfold ϕ_sem, ϕ_plug in *. destruct H as [m [es [hp H]]].
+  now rewrite hp. 
 Qed.
 
 Axiom some_ctx_L : ctx L.
@@ -251,10 +298,9 @@ Proof.
     simpl in ff.
     assert (hh :  (forall (C : ctx ϕ) (t : trace), sem ϕ (ϕ_plug P C) t -> my_pi t)).
     { intros C t H0. simpl in H0. unfold ϕ_sem, ϕ_plug in H0.
-      destruct H0 as [m [e [hm H0]]]. left. rewrite hm.
-      now apply embed_fin. }
-    specialize (ff my_pi_liveness hh).  specialize (ff some_ctx_L another_omega).
-    assert (sem L (some_ctx_L [P]) another_omega) by now apply (H some_ctx_L).
+      destruct H0 as [m [e [hm H0]]]. now rewrite hm. }
+    specialize (ff my_pi_liveness hh).  specialize (ff some_ctx_L (tstream another_omega)).
+    assert (sem L (some_ctx_L [P]) (tstream another_omega)) by now apply (H some_ctx_L).
     specialize (ff H0). now apply another_omega_not_in_my_pi.
 Qed.
 
